Interacction with Steel
+ use Type0 instead of prop
+ provide an alternative selector for vprop_list, proved equal modulo
  exposing the definition of valid_rmem

experiment/Experiment.Steel.Repr.M.fst
@@ -82,12 +82,73 @@ let rec vprop_equiv_flat (vp : vprop)
                               (v0 `star` v1)
 
 
+let sel'_sub (#p : vprop) (vs : vprop_list)
+             (h : rmem p{can_be_split p (vprop_of_list vs)})
+  : sl_t vs
+  = sel' vs (focus_rmem h (vprop_of_list vs))
+
+let rmem_star_eq (#p : vprop) (v0 v1 : vprop)
+      (h : rmem p{can_be_split p (VStar v0 v1)})
+  : Lemma (can_be_split p v0 /\ can_be_split p v1 /\
+           h (VStar v0 v1) == (h v0, h v1))
+  =
+    can_be_split_star_l v0 v1;
+    can_be_split_star_r v0 v1;
+    can_be_split_trans p (VStar v0 v1) v0;
+    can_be_split_trans p (VStar v0 v1) v1;
+    // TODO: this is implied by [valid_rmem] but not exposed by the interface of [Steel.Effect.Common]
+    //       maybe we can do the proofs in SteelGhost
+    admit ()
+
+let focus_rmem_feq (p q r : vprop) (h : rmem p)
+  : Lemma (requires can_be_split p q /\ can_be_split q r)
+          (ensures  can_be_split p r /\ focus_rmem h q r == h r)
+  = can_be_split_trans p q r
+
+#push-options "--ifuel 1 --fuel 1"
+let rec sel_list_eq'_sub (#p : vprop) (vs : vprop_list)
+                    (h : rmem p{can_be_split p (vprop_of_list vs)})
+  : Lemma (sel_list' #p vs h == Fl.dlist_of_f_g (sel'_sub #p vs h))
+  = match vs with
+  | [] -> ()
+  | v0 :: vs ->
+       rmem_star_eq (VUnit v0) (vprop_of_list vs) h;
+       calc (==) {
+         sel_list' #p (v0 :: vs) h;
+       == {}
+         Dl.DCons v0.t (h (VUnit v0)) _ (sel_list' #p vs h);
+       == { sel_list_eq'_sub #p vs h }
+         Dl.DCons v0.t (h (VUnit v0)) _ (Fl.dlist_of_f_g (sel'_sub #p vs h));
+       == { Dl.dlist_extensionality
+              (Dl.DCons v0.t (h (VUnit v0)) _ (Fl.dlist_of_f_g (sel'_sub #p vs h)))
+              (Fl.dlist_of_f_g (sel'_sub #p (v0 :: vs) h))
+              (fun i -> vprop_of_list_can_be_split (v0 :: vs) i;
+                     focus_rmem_feq p (vprop_of_list (v0 :: vs)) (VUnit (L.index (v0 :: vs) i)) h;
+                     if i > 0 then begin
+                       vprop_of_list_can_be_split vs (i - 1);
+                       focus_rmem_feq p (vprop_of_list vs) (VUnit (L.index vs (i - 1))) h
+                     end ) }
+         Fl.dlist_of_f_g (sel'_sub #p (v0 :: vs) h);
+       }
+#pop-options
+
+let sel_list_eq' (vs : vprop_list) (h : rmem (vprop_of_list vs))
+  : Lemma (sel_list vs h == Fl.dlist_of_f_g (sel' vs h))
+  = sel_list_eq'_sub vs h;
+    focus_rmem_refl (vprop_of_list vs) h
+
+let sel_eq' : squash (sel == sel_f')
+  = U.funext_eta sel_f' sel (_ by T.(trefl ())) (_ by T.(trefl ())) (fun vs ->
+    U.funext_eta_gtot (sel_f' vs) (sel vs) (_ by T.(trefl ())) (_ by T.(trefl ())) (fun h ->
+      sel_f_eq' vs h))
+
+
 let rec steel_elim_vprop_of_list_append #opened (vs0 vs1 : vprop_list)
   : SteelGhost unit opened
       (vprop_of_list L.(vs0@vs1)) (fun () -> vprop_of_list vs0 `star` vprop_of_list vs1)
       (requires fun _ -> True)
-      (ensures fun h0 () h1 -> split_vars_list vs0 vs1 (rmem_sl_list (vs0@vs1) h0)
-                        == (rmem_sl_list vs0 h1, rmem_sl_list vs1 h1))
+      (ensures fun h0 () h1 -> split_vars_list vs0 vs1 (sel_list (vs0@vs1) h0)
+                        == (sel_list vs0 h1, sel_list vs1 h1))
       (decreases %[vs0; 0])
   =
     match vs0 with
@@ -99,8 +160,8 @@ and steel_elim_vprop_of_list_append__cons #opened (vs0 vs1 : vprop_list) v0 (vs0
   : SteelGhost unit opened
       (vprop_of_list L.(vs0@vs1)) (fun () -> vprop_of_list vs0 `star` vprop_of_list vs1)
       (requires fun _ -> vs0 == v0 :: vs0')
-      (ensures fun h0 () h1 -> split_vars_list vs0 vs1 (rmem_sl_list (vs0@vs1) h0)
-                        == (rmem_sl_list vs0 h1, rmem_sl_list vs1 h1))
+      (ensures fun h0 () h1 -> split_vars_list vs0 vs1 (sel_list (vs0@vs1) h0)
+                        == (sel_list vs0 h1, sel_list vs1 h1))
       (decreases %[vs0'; 1])
   =
     change_equal_slprop (vprop_of_list L.(vs0@vs1)) (VUnit v0 `star` vprop_of_list L.(vs0'@vs1));
@@ -123,8 +184,8 @@ let steel_elim_vprop_of_list_append_f #opened (vs0 vs1 : vprop_list)
   : SteelGhost unit opened
       (vprop_of_list L.(vs0@vs1)) (fun () -> vprop_of_list vs0 `star` vprop_of_list vs1)
       (requires fun _ -> True)
-      (ensures fun h0 () h1 -> split_vars vs0 vs1 (rmem_sels (vs0@vs1) h0)
-                        == (rmem_sels vs0 h1, rmem_sels vs1 h1))
+      (ensures fun h0 () h1 -> split_vars vs0 vs1 (sel_f (vs0@vs1) h0)
+                        == (sel_f vs0 h1, sel_f vs1 h1))
   =
     let sl = gget (vprop_of_list L.(vs0@vs1)) in
     Ll.map_append Mkvprop'?.t vs0 vs1;
@@ -139,8 +200,8 @@ let rec steel_intro_vprop_of_list_append #opened (vs0 vs1 : vprop_list)
   : SteelGhost unit opened
       (vprop_of_list vs0 `star` vprop_of_list vs1) (fun () -> vprop_of_list L.(vs0@vs1))
       (requires fun _ -> True)
-      (ensures fun h0 () h1 -> split_vars_list vs0 vs1 (rmem_sl_list (vs0@vs1) h1)
-                        == (rmem_sl_list vs0 h0, rmem_sl_list vs1 h0))
+      (ensures fun h0 () h1 -> split_vars_list vs0 vs1 (sel_list (vs0@vs1) h1)
+                        == (sel_list vs0 h0, sel_list vs1 h0))
       (decreases vs0)
   = match vs0 with
     | [] -> change_equal_slprop (vprop_of_list vs0) emp;
@@ -157,8 +218,8 @@ let steel_intro_vprop_of_list_append_f #opened (vs0 vs1 : vprop_list)
   : SteelGhost unit opened
       (vprop_of_list vs0 `star` vprop_of_list vs1) (fun () -> vprop_of_list L.(vs0@vs1))
       (requires fun _ -> True)
-      (ensures fun h0 () h1 -> split_vars vs0 vs1 (rmem_sels (vs0@vs1) h1)
-                        == (rmem_sels vs0 h0, rmem_sels vs1 h0))
+      (ensures fun h0 () h1 -> split_vars vs0 vs1 (sel_f (vs0@vs1) h1)
+                        == (sel_f vs0 h0, sel_f vs1 h0))
   =
     steel_intro_vprop_of_list_append vs0 vs1;
     let sl = gget (vprop_of_list L.(vs0@vs1)) in
@@ -174,7 +235,7 @@ let rec steel_change_swap (#opened:Mem.inames)
           (vs0 : vprop_list) (i : nat {i <= L.length vs0 - 2})
   : SteelGhost unit opened (vprop_of_list vs0) (fun () -> vprop_of_list (Perm.list_swap i vs0))
       (requires fun _ -> True) (ensures fun h0 () h1 ->
-        rmem_sl_list (Perm.list_swap i vs0) h1 === Dl.dlist_swap i (rmem_sl_list vs0 h0))
+        sel_list (Perm.list_swap i vs0) h1 === Dl.dlist_swap i (sel_list vs0 h0))
       (decreases i)
   = if i = 0
     then begin
@@ -198,8 +259,8 @@ let rec steel_change_vequiv_aux (#opened:Mem.inames)
           (eqv : squash (vs1 == Perm.apply_perm_r (Perm.comp_list (L.map (Perm.perm_f_swap #n) fs)) vs0))
   : SteelGhost unit opened (vprop_of_list vs0) (fun () -> vprop_of_list vs1)
       (requires fun _ -> True) (ensures fun h0 () h1 ->
-        rmem_sl_list vs1 h1 == Dl.apply_pequiv (vequiv_sl (Perm.comp_list (L.map Perm.perm_f_swap fs)))
-                                            (rmem_sl_list vs0 h0))
+        sel_list vs1 h1 == Dl.apply_pequiv (vequiv_sl (Perm.comp_list (L.map Perm.perm_f_swap fs)))
+                                           (sel_list vs0 h0))
       (decreases fs)
   =
   let sl0  = gget (vprop_of_list vs0) in
@@ -225,7 +286,7 @@ let rec steel_change_vequiv_aux (#opened:Mem.inames)
 let steel_change_vequiv (#vs0 #vs1 : vprop_list) (#opened:Mem.inames) (f : vequiv vs0 vs1)
   : SteelGhost unit opened (vprop_of_list vs0) (fun () -> vprop_of_list vs1)
       (requires fun _ -> True)
-      (ensures fun h0 () h1 -> rmem_sels vs1 h1 == extract_vars f (rmem_sels vs0 h0))
+      (ensures fun h0 () h1 -> sel_f vs1 h1 == extract_vars f (sel_f vs0 h0))
   =
     let sl0 = gget (vprop_of_list vs0) in
     Fl.apply_perm_r_of_d f (vpl_sels vs0 sl0);
@@ -245,7 +306,7 @@ let elim_tree_req_bind (#a #b : Type) (f : prog_tree a) (g : a -> prog_tree b)
                       tree_req (g x) (cg x) (vpl_sels_f (itm x) sl1)))
   = assert_norm (tree_req _ (TCbind #a #b #f #g pre itm post cf cg) (vpl_sels_f pre sl0) == (
       tree_req f cf (vpl_sels_f pre sl0) /\
-      (forall (x : a) (sl1 : sl_t (itm x)) .
+      (forall (x : a) (sl1 : sl_f (itm x)) .
          tree_ens f cf (vpl_sels_f pre sl0) x sl1 ==> tree_req (g x) (cg x) sl1)
     ))
 
@@ -261,7 +322,7 @@ let intro_tree_ens_bind (#a #b : Type) (f : prog_tree a) (g : a -> prog_tree b)
                              (vpl_sels_f pre sl0) y (vpl_sels_f (post y) sl2))
   = assert_norm (tree_ens _ (TCbind #a #b #f #g pre itm post cf cg)
                           (vpl_sels_f pre sl0) y (vpl_sels_f (post y) sl2) == (
-        (exists (x : a) (sl1 : sl_t (itm x)) .
+        (exists (x : a) (sl1 : sl_f (itm x)) .
           tree_ens f cf (vpl_sels_f pre sl0) x sl1 /\
           tree_ens (g x) (cg x) sl1 y (vpl_sels_f (post y) sl2))
     ))
