experiment/Experiment.Steel.Repr.Test.Extract.fst
@@ -12,7 +12,7 @@ let test3 (r0 r1 : ref U32.t)
   : Steel unit
       (M.vprop_of_list (Test.test3_mem r0 r1)) (fun x -> M.vprop_of_list (Test.test3_mem r0 r1))
       (requires fun h0      ->
-        U32.v (M.rmem_sels (Test.test3_mem r0 r1) h0 0) < 42)
+        U32.v (M.sel_f (Test.test3_mem r0 r1) h0 0) < 42)
       (ensures  fun h0 () h1 ->
-        U32.v (M.rmem_sels (Test.test3_mem r0 r1) h1 1) == U32.v (M.rmem_sels (Test.test3_mem r0 r1) h0 0) + 1)
+        U32.v (M.sel_f (Test.test3_mem r0 r1) h1 1) == U32.v (M.sel_f (Test.test3_mem r0 r1) h0 0) + 1)
   = Test.test3_steel r0 r1 ()
